fixes to a working version

theories/iris.v
@@ -31,7 +31,7 @@ Let reduce : host_state -> store_record -> frame -> list administrative_instruct
 
 Definition expr := list administrative_instruction.
 Definition val := list value.
-Definition state : Type := host_state * store_record.
+Definition state : Type := host_state * store_record * (list value).
 Definition observation := unit. (* TODO: maybe change? *)
 
 Definition of_val (v : val) : expr := fmap (fun v => AI_basic (BI_const v)) v.
@@ -48,12 +48,10 @@ Fixpoint to_val (e : expr) : option val :=
   end.
 
 Definition prim_step (e : expr) (s : state) (os : list observation) (e' : expr) (s' : state) (fork_es' : list expr) : Prop :=
-  let '(hs, σ) := s in
-  let '(hs', σ') := s' in
-  let '(vs, es) := split_vals_e e in
-  let '(vs', es') := split_vals_e e' in
+  let '(hs, σ, locs) := s in
+  let '(hs', σ', locs') := s' in
   exists i,
-    reduce hs σ (Build_frame vs i) es hs' σ' (Build_frame vs' i) es' /\ os = [] /\ fork_es' = [].
+    reduce hs σ (Build_frame locs i) e hs' σ' (Build_frame locs' i) e' /\ os = [] /\ fork_es' = [].
 
 Lemma to_of_val v : to_val (of_val v) = Some v.
 Proof.
@@ -131,6 +129,18 @@ Proof.
   rewrite (IH _ _ _ H1).
   done.
 Qed.
+
+Lemma to_val_None_prepend: forall es1 es2,
+  to_val es2 = None ->
+  to_val (es1 ++ es2) = None.
+Proof.
+Admitted.
+  
+Lemma to_val_None_append: forall es1 es2,
+  to_val es1 = None ->
+  to_val (es1 ++ es2) = None.
+Proof.
+Admitted.
 
 Lemma cat_cons_not_nil : forall T (xs : list T) y ys,
   xs ++ (y :: ys) <> [].
@@ -234,19 +244,19 @@ Lemma val_head_stuck : forall e1 s1 κ e2 s2 efs,
   prim_step e1 s1 κ e2 s2 efs →
   to_val e1 = None.
 Proof.
-  rewrite /prim_step => e1 [hs1 σ1] κ e2 [hs2 σ2] efs.
-  case_eq (split_vals_e e1) => vs es H.
-  case_eq (split_vals_e e2) => vs' es' _ [i [Hred _]].
-  move: vs vs' es' H Hred.
-  elim: es.
-  { move => vs vs' es' _ Hred.
-    exfalso.
-    apply: reduce_not_nil.
-    apply: Hred.
-    done. }
-  { move => e es _ vs vs' _ H1 _ {e2 efs}.
-    apply: splits_vals_e_to_val_hd.
-    apply: H1. }
+  rewrite /prim_step => e1 [[hs1 locs1] σ1] κ e2 [[hs2 locs2] σ2] efs.
+  move => [i [HRed _]].
+  induction HRed => //=; subst; try by apply to_val_None_prepend.
+  - inversion H; subst => //=; try by apply to_val_None_prepend.
+    + destruct v => //=.
+      by destruct b => //=.
+    + move/lfilledP in H1.
+      inversion H1; subst; clear H1.
+      by apply to_val_None_prepend, to_val_None_append. 
+  - move/lfilledP in H.
+    inversion H; subst; clear H.
+    by apply to_val_None_prepend, to_val_None_append.
+  - by apply to_val_None_prepend, to_val_None_append.
 Qed.
 
 Lemma wasm_mixin : LanguageMixin of_val to_val prim_step.
